backend/Linearizeproof.v
@@ -24,11 +24,10 @@ Module NodesetFacts := FSetFacts.Facts(Nodeset).
 Definition match_prog (p: LTL.program) (tp: Linear.program) :=
   match_program (fun ctx f tf => transf_fundef f = OK tf) eq p tp.
 
-Instance comp_transf_fundef P:
-  has_comp_match (fun (ctx: P) f tf => transf_fundef f = OK tf).
+Instance comp_transf_fundef: has_comp_transl_partial transf_fundef.
 Proof.
   unfold transf_fundef, transf_function.
-  intros cu [f|ef] ? H; monadInv H; trivial.
+  intros [f|ef] ? H; monadInv H; trivial.
   now monadInv EQ.
 Qed.
 
