backend/RTLgenproof.v
@@ -351,11 +351,10 @@ Require Import Errors.
 Definition match_prog (p: CminorSel.program) (tp: RTL.program) :=
   match_program (fun cu f tf => transl_fundef f = Errors.OK tf) eq p tp.
 
-Instance comp_transl_function P:
-  has_comp_match (fun (cu : P) f tf => transl_fundef f = Errors.OK tf).
+Instance comp_transl_function: has_comp_transl_partial transl_fundef.
 Proof.
   unfold transl_fundef, transf_partial_fundef, transl_function.
-  intros cu [f|?] tf H; simpl; monadInv H; trivial.
+  intros [f|?] tf H; simpl; monadInv H; trivial.
   destruct (reserve_labels _ _) as [l s].
   destruct (transl_fun _ _ _) as [|[??] ? ?]; try discriminate.
   now monadInv EQ.
