backend/Stackingproof.v
@@ -26,11 +26,10 @@ Local Open Scope sep_scope.
 Definition match_prog (p: Linear.program) (tp: Mach.program) :=
   match_program (fun _ f tf => transf_fundef f = OK tf) eq p tp.
 
-Instance comp_transf_fundef P:
-  has_comp_match (fun (_: P) f tf => transf_fundef f = OK tf).
+Instance comp_transf_fundef: has_comp_transl_partial transf_fundef.
 Proof.
   unfold transf_fundef, transf_function.
-  intros _ [f|ef] tf H; monadInv H; trivial.
+  intros [f|ef] tf H; monadInv H; trivial.
   destruct negb; try easy.
   destruct zlt; try easy.
   now monadInv EQ.
